include/s2n-bignum.h
@@ -241,6 +241,10 @@ extern void bignum_double_p384 (uint64_t z[static 6], uint64_t x[static 6]);
 // Input x[9]; output z[9]
 extern void bignum_double_p521 (uint64_t z[static 9], uint64_t x[static 9]);
 
+// Double modulo p_sm2, z := (2 * x) mod p_sm2, assuming x reduced
+// Input x[4]; output z[4]
+extern void bignum_double_sm2 (uint64_t z[static 4], uint64_t x[static 4]);
+
 // Extended Montgomery reduce, returning results in input-output buffer
 // Inputs z[2*k], m[k], w; outputs function return (extra result bit) and z[2*k]
 extern uint64_t bignum_emontredc (uint64_t k, uint64_t *z, uint64_t *m, uint64_t w);
@@ -300,6 +304,10 @@ extern void bignum_half_p384 (uint64_t z[static 6], uint64_t x[static 6]);
 // Halve modulo p_521, z := (x / 2) mod p_521, assuming x reduced
 // Input x[9]; output z[9]
 extern void bignum_half_p521 (uint64_t z[static 9], uint64_t x[static 9]);
+
+// Halve modulo p_sm2, z := (x / 2) mod p_sm2, assuming x reduced
+// Input x[4]; output z[4]
+extern void bignum_half_sm2 (uint64_t z[static 4], uint64_t x[static 4]);
 
 // Test bignum for zero-ness, x = 0
 // Input x[k]; output function return
