arm/proofs/bignum_half_sm2.ml
@@ -4,90 +4,83 @@
  *)
 
 (* ========================================================================= *)
-(* Halving modulo p_384, the field characteristic for the NIST P-384 curve.  *)
+(* Halving modulo p_sm2, the field characteristic for the CC SM2 curve.      *)
 (* ========================================================================= *)
 
-(**** print_literal_from_elf "arm/p384/bignum_half_p384.o";;
+(**** print_literal_from_elf "arm/sm2/bignum_half_sm2.o";;
  ****)
 
-let bignum_half_p384_mc = define_assert_from_elf "bignum_half_p384_mc" "arm/p384/bignum_half_p384.o"
+let bignum_half_sm2_mc = define_assert_from_elf "bignum_half_sm2_mc" "arm/sm2/bignum_half_sm2.o"
 [
   0xa9400c22;       (* arm_LDP X2 X3 X1 (Immediate_Offset (iword (&0))) *)
   0xa9411424;       (* arm_LDP X4 X5 X1 (Immediate_Offset (iword (&16))) *)
-  0xa9421c26;       (* arm_LDP X6 X7 X1 (Immediate_Offset (iword (&32))) *)
-  0x9240004a;       (* arm_AND X10 X2 (rvalue (word 1)) *)
-  0xcb0a03ea;       (* arm_NEG X10 X10 *)
-  0x92407d4b;       (* arm_AND X11 X10 (rvalue (word 4294967295)) *)
-  0xab0b0042;       (* arm_ADDS X2 X2 X11 *)
-  0x92607d4b;       (* arm_AND X11 X10 (rvalue (word 18446744069414584320)) *)
-  0xba0b0063;       (* arm_ADCS X3 X3 X11 *)
-  0x927ff94b;       (* arm_AND X11 X10 (rvalue (word 18446744073709551614)) *)
-  0xba0b0084;       (* arm_ADCS X4 X4 X11 *)
-  0xba0a00a5;       (* arm_ADCS X5 X5 X10 *)
-  0xba0a00c6;       (* arm_ADCS X6 X6 X10 *)
-  0xba0a00e7;       (* arm_ADCS X7 X7 X10 *)
-  0x9a1f03e8;       (* arm_ADC X8 XZR XZR *)
+  0x92400047;       (* arm_AND X7 X2 (rvalue (word 1)) *)
+  0xcb0703e7;       (* arm_NEG X7 X7 *)
+  0xab070042;       (* arm_ADDS X2 X2 X7 *)
+  0x92607ce8;       (* arm_AND X8 X7 (rvalue (word 18446744069414584320)) *)
+  0xba080063;       (* arm_ADCS X3 X3 X8 *)
+  0xba070084;       (* arm_ADCS X4 X4 X7 *)
+  0x925ff8e8;       (* arm_AND X8 X7 (rvalue (word 18446744069414584319)) *)
+  0xba0800a5;       (* arm_ADCS X5 X5 X8 *)
+  0x9a1f03e6;       (* arm_ADC X6 XZR XZR *)
   0x93c20462;       (* arm_EXTR X2 X3 X2 1 *)
   0x93c30483;       (* arm_EXTR X3 X4 X3 1 *)
   0x93c404a4;       (* arm_EXTR X4 X5 X4 1 *)
   0x93c504c5;       (* arm_EXTR X5 X6 X5 1 *)
-  0x93c604e6;       (* arm_EXTR X6 X7 X6 1 *)
-  0x93c70507;       (* arm_EXTR X7 X8 X7 1 *)
   0xa9000c02;       (* arm_STP X2 X3 X0 (Immediate_Offset (iword (&0))) *)
   0xa9011404;       (* arm_STP X4 X5 X0 (Immediate_Offset (iword (&16))) *)
-  0xa9021c06;       (* arm_STP X6 X7 X0 (Immediate_Offset (iword (&32))) *)
   0xd65f03c0        (* arm_RET X30 *)
 ];;
 
-let BIGNUM_HALF_P384_EXEC = ARM_MK_EXEC_RULE bignum_half_p384_mc;;
+let BIGNUM_HALF_SM2_EXEC = ARM_MK_EXEC_RULE bignum_half_sm2_mc;;
 
 (* ------------------------------------------------------------------------- *)
 (* Proof.                                                                    *)
 (* ------------------------------------------------------------------------- *)
 
-let p_384 = new_definition `p_384 = 39402006196394479212279040100143613805079739270465446667948293404245721771496870329047266088258938001861606973112319`;;
+let p_sm2 = new_definition `p_sm2 = 0xFFFFFFFEFFFFFFFFFFFFFFFFFFFFFFFFFFFFFFFF00000000FFFFFFFFFFFFFFFF`;;
 
-let BIGNUM_HALF_P384_CORRECT = time prove
+let BIGNUM_HALF_SM2_CORRECT = time prove
  (`!z x n pc.
-        nonoverlapping (word pc,0x64) (z,8 * 6)
+        nonoverlapping (word pc,0x48) (z,8 * 4)
         ==> ensures arm
-             (\s. aligned_bytes_loaded s (word pc) bignum_half_p384_mc /\
+             (\s. aligned_bytes_loaded s (word pc) bignum_half_sm2_mc /\
                   read PC s = word pc /\
                   C_ARGUMENTS [z; x] s /\
-                  bignum_from_memory (x,6) s = n)
-             (\s. read PC s = word (pc + 0x60) /\
-                  (n < p_384
-                   ==> bignum_from_memory (z,6) s =
-                       (inverse_mod p_384 2 * n) MOD p_384))
-          (MAYCHANGE [PC; X2; X3; X4; X5; X6; X7; X8; X9; X10; X11] ,,
+                  bignum_from_memory (x,4) s = n)
+             (\s. read PC s = word (pc + 0x44) /\
+                  (n < p_sm2
+                   ==> bignum_from_memory (z,4) s =
+                       (inverse_mod p_sm2 2 * n) MOD p_sm2))
+          (MAYCHANGE [PC; X2; X3; X4; X5; X6; X7; X8] ,,
            MAYCHANGE SOME_FLAGS ,,
-           MAYCHANGE [memory :> bignum(z,6)])`,
+           MAYCHANGE [memory :> bignum(z,4)])`,
   MAP_EVERY X_GEN_TAC
    [`z:int64`; `x:int64`; `n:num`; `pc:num`] THEN
   REWRITE_TAC[C_ARGUMENTS; C_RETURN; SOME_FLAGS; NONOVERLAPPING_CLAUSES] THEN
   DISCH_THEN(REPEAT_TCL CONJUNCTS_THEN ASSUME_TAC) THEN
   REWRITE_TAC[BIGNUM_FROM_MEMORY_BYTES] THEN ENSURES_INIT_TAC "s0" THEN
-  BIGNUM_DIGITIZE_TAC "n_" `read (memory :> bytes (x,8 * 6)) s0` THEN
+  BIGNUM_DIGITIZE_TAC "n_" `read (memory :> bytes (x,8 * 4)) s0` THEN
 
-  ARM_STEPS_TAC BIGNUM_HALF_P384_EXEC (1--6) THEN
+  ARM_STEPS_TAC BIGNUM_HALF_SM2_EXEC (1--4) THEN
   RULE_ASSUM_TAC(REWRITE_RULE[WORD_SUB_LZERO; WORD_AND_1_BITVAL]) THEN
   SUBGOAL_THEN `bit 0 (n_0:int64) <=> ODD n` SUBST_ALL_TAC THENL
    [EXPAND_TAC "n" THEN REWRITE_TAC[BIT_LSB; ODD_ADD; ODD_MULT; ODD_EXP] THEN
     CONV_TAC NUM_REDUCE_CONV;
     ALL_TAC] THEN
-  ARM_ACCSTEPS_TAC BIGNUM_HALF_P384_EXEC (7--14) (7--24) THEN
+  ARM_ACCSTEPS_TAC BIGNUM_HALF_SM2_EXEC (5--11) (5--17) THEN
   ENSURES_FINAL_STATE_TAC THEN ASM_REWRITE_TAC[] THEN STRIP_TAC THEN
 
   SUBGOAL_THEN
-   `(inverse_mod p_384 2 * n) MOD p_384 =
-    (if ODD n then n + p_384 else n) DIV 2`
+   `(inverse_mod p_sm2 2 * n) MOD p_sm2 =
+    (if ODD n then n + p_sm2 else n) DIV 2`
   SUBST1_TAC THENL
    [REWRITE_TAC[MOD_UNIQUE] THEN CONJ_TAC THENL
-     [DISJ2_TAC THEN UNDISCH_TAC `n < p_384` THEN ARITH_TAC; ALL_TAC] THEN
+     [DISJ2_TAC THEN UNDISCH_TAC `n < p_sm2` THEN ARITH_TAC; ALL_TAC] THEN
     ONCE_REWRITE_TAC[CONG_SYM] THEN MATCH_MP_TAC CONG_DIV_COPRIME THEN
     REWRITE_TAC[COPRIME_2; DIVIDES_2; GSYM NOT_ODD] THEN
     ONCE_REWRITE_TAC[COND_RAND] THEN
-    SIMP_TAC[p_384; ODD_ADD] THEN CONV_TAC NUM_REDUCE_CONV THEN
+    SIMP_TAC[p_sm2; ODD_ADD] THEN CONV_TAC NUM_REDUCE_CONV THEN
     REWRITE_TAC[COND_ID] THEN REWRITE_TAC[COND_RATOR; COND_RAND] THEN
     REWRITE_TAC[COND_ID; NUMBER_RULE
      `(n + p:num == m) (mod p) <=> (n == m) (mod p)`] THEN
@@ -96,11 +89,11 @@ let BIGNUM_HALF_P384_CORRECT = time prove
     REWRITE_TAC[INVERSE_MOD_RMUL_EQ; COPRIME_2] THEN CONV_TAC NUM_REDUCE_CONV;
     ALL_TAC] THEN
   SUBGOAL_THEN
-   `2 EXP 384 * bitval(carry_s14) +
-    bignum_of_wordlist [sum_s7; sum_s9; sum_s11; sum_s12; sum_s13; sum_s14] =
-    if ODD n then n + p_384 else n`
+   `2 EXP 256 * bitval(carry_s10) +
+    bignum_of_wordlist [sum_s5; sum_s7; sum_s8; sum_s10] =
+    if ODD n then n + p_sm2 else n`
   (SUBST1_TAC o SYM) THENL
-   [REWRITE_TAC[GSYM REAL_OF_NUM_CLAUSES; bignum_of_wordlist; p_384] THEN
+   [REWRITE_TAC[GSYM REAL_OF_NUM_CLAUSES; bignum_of_wordlist; p_sm2] THEN
     ASM_REWRITE_TAC[] THEN
     ACCUMULATOR_ASSUM_LIST(MP_TAC o end_itlist CONJ o DESUM_RULE) THEN
     COND_CASES_TAC THEN
@@ -110,28 +103,28 @@ let BIGNUM_HALF_P384_CORRECT = time prove
     DISCH_THEN(fun th -> REWRITE_TAC[th]) THEN REAL_ARITH_TAC;
     ALL_TAC] THEN
   CONV_TAC(LAND_CONV BIGNUM_EXPAND_CONV) THEN
-  ASM_REWRITE_TAC[] THEN DISCARD_STATE_TAC "s24" THEN
+  ASM_REWRITE_TAC[] THEN DISCARD_STATE_TAC "s21" THEN
   REWRITE_TAC[DIMINDEX_64] THEN CONV_TAC(ONCE_DEPTH_CONV NUM_MOD_CONV) THEN
   REWRITE_TAC[MATCH_MP VAL_WORD_SUBWORD_JOIN_64 (ARITH_RULE `1 <= 64`)] THEN
   SIMP_TAC[VAL_WORD_BITVAL; ADD_CLAUSES; bignum_of_wordlist; MULT_CLAUSES;
            BITVAL_BOUND_ALT; MOD_LT; EXP_1] THEN
   ARITH_TAC);;
 
-let BIGNUM_HALF_P384_SUBROUTINE_CORRECT = time prove
+let BIGNUM_HALF_SM2_SUBROUTINE_CORRECT = time prove
  (`!z x n pc returnaddress.
-        nonoverlapping (word pc,0x64) (z,8 * 6)
+        nonoverlapping (word pc,0x48) (z,8 * 4)
         ==> ensures arm
-             (\s. aligned_bytes_loaded s (word pc) bignum_half_p384_mc /\
+             (\s. aligned_bytes_loaded s (word pc) bignum_half_sm2_mc /\
                   read PC s = word pc /\
                   read X30 s = returnaddress /\
                   C_ARGUMENTS [z; x] s /\
-                  bignum_from_memory (x,6) s = n)
+                  bignum_from_memory (x,4) s = n)
              (\s. read PC s = returnaddress /\
-                  (n < p_384
-                   ==> bignum_from_memory (z,6) s =
-                       (inverse_mod p_384 2 * n) MOD p_384))
-          (MAYCHANGE [PC; X2; X3; X4; X5; X6; X7; X8; X9; X10; X11] ,,
+                  (n < p_sm2
+                   ==> bignum_from_memory (z,4) s =
+                       (inverse_mod p_sm2 2 * n) MOD p_sm2))
+          (MAYCHANGE [PC; X2; X3; X4; X5; X6; X7; X8] ,,
            MAYCHANGE SOME_FLAGS ,,
-           MAYCHANGE [memory :> bignum(z,6)])`,
-  ARM_ADD_RETURN_NOSTACK_TAC BIGNUM_HALF_P384_EXEC
-    BIGNUM_HALF_P384_CORRECT);;
+           MAYCHANGE [memory :> bignum(z,4)])`,
+  ARM_ADD_RETURN_NOSTACK_TAC BIGNUM_HALF_SM2_EXEC
+    BIGNUM_HALF_SM2_CORRECT);;
